theory bitvector_examples_Test_imperial_violet_addqtvc
  imports "NTP4Verif.NTP4Verif" "Why3STD.WellFounded_WellFounded"
begin
theorem add'vc:
  fixes a :: "32 word list"
  fixes b :: "32 word list"
  assumes fact0: "length a = length b"
  assumes fact1: "\<forall>(i :: int). (0 :: int) \<le> i \<and> i < int (length a) \<longrightarrow> a ! nat i < (2147483648 :: 32 word)"
  assumes fact2: "\<forall>(i :: int). (0 :: int) \<le> i \<and> i < int (length b) \<longrightarrow> b ! nat i < (2147483648 :: 32 word)"
  shows "let o1 :: int = int (length a) in (0 :: int) \<le> o1 \<and> (\<forall>(sum :: 32 word list). (\<forall>(i :: int). (0 :: int) \<le> i \<and> i < o1 \<longrightarrow> sum ! nat i = (0 :: 32 word)) \<and> int (length sum) = o1 \<longrightarrow> (let o2 :: int = int (length a) - (1 :: int) in ((0 :: int) \<le> o2 + (1 :: int) \<longrightarrow> ((\<forall>(j :: int). (0 :: int) \<le> j \<and> j < (0 :: int) \<longrightarrow> sum ! nat j = a ! nat j + b ! nat j) \<and> (\<forall>(j :: int). (0 :: int) \<le> j \<and> j < (0 :: int) \<longrightarrow> uint (sum ! nat j) = uint (a ! nat j) + uint (b ! nat j))) \<and> (\<forall>(sum1 :: 32 word list). length sum1 = length sum \<longrightarrow> (\<forall>(i :: int). ((0 :: int) \<le> i \<and> i \<le> o2) \<and> (\<forall>(j :: int). (0 :: int) \<le> j \<and> j < i \<longrightarrow> sum1 ! nat j = a ! nat j + b ! nat j) \<and> (\<forall>(j :: int). (0 :: int) \<le> j \<and> j < i \<longrightarrow> uint (sum1 ! nat j) = uint (a ! nat j) + uint (b ! nat j)) \<longrightarrow> ((0 :: int) \<le> i \<and> i < int (length b)) \<and> ((0 :: int) \<le> i \<and> i < int (length a)) \<and> (let o3 :: 32 word = a ! nat i + b ! nat i in ((0 :: int) \<le> i \<and> i < int (length sum1)) \<and> (length (sum1[nat i := o3]) = length sum1 \<longrightarrow> nth (sum1[nat i := o3]) o nat = (nth sum1 o nat)(i := o3) \<longrightarrow> (\<forall>(j :: int). (0 :: int) \<le> j \<and> j < i + (1 :: int) \<longrightarrow> sum1[nat i := o3] ! nat j = a ! nat j + b ! nat j) \<and> (\<forall>(j :: int). (0 :: int) \<le> j \<and> j < i + (1 :: int) \<longrightarrow> uint (sum1[nat i := o3] ! nat j) = uint (a ! nat j) + uint (b ! nat j))))) \<and> ((\<forall>(j :: int). (0 :: int) \<le> j \<and> j < o2 + (1 :: int) \<longrightarrow> sum1 ! nat j = a ! nat j + b ! nat j) \<and> (\<forall>(j :: int). (0 :: int) \<le> j \<and> j < o2 + (1 :: int) \<longrightarrow> uint (sum1 ! nat j) = uint (a ! nat j) + uint (b ! nat j)) \<longrightarrow> (\<forall>(i :: int). (0 :: int) \<le> i \<and> i < int (length sum1) \<longrightarrow> uint (sum1 ! nat i) = uint (a ! nat i) + uint (b ! nat i))))) \<and> (o2 + (1 :: int) < (0 :: int) \<longrightarrow> (\<forall>(i :: int). (0 :: int) \<le> i \<and> i < int (length sum) \<longrightarrow> uint (sum ! nat i) = uint (a ! nat i) + uint (b ! nat i)))))"
  sorry
end
