theory my_strassen_MatrixMultiplication_subqtvc
  imports "NTP4Verif.NTP4Verif" "Why3STD.Ref_Ref" "Why3STD.int_Sum" "../../lib/isabelle/matrices_MyMatrix" "../../lib/isabelle/matrices_MatrixArithmetic" "../../lib/isabelle/sum_extended_Sum_extended" "../../lib/isabelle/matrices_BlockMul" "../../lib/isabelle/matrices_ring_simp_Symb" "Why3STD.matrix_Matrix"
begin
definition mdl :: "'a matrix \<Rightarrow> 'a mat"
  where "mdl m = create (matrix_Matrix.rows m) (columns m) (elts m)" for m
datatype  with_symb = with_symb'mk (phy: "int matrix") (sym: "expr")
definition with_symb_vld :: "env \<Rightarrow> with_symb \<Rightarrow> _"
  where "with_symb_vld env ws \<longleftrightarrow> e_mdl env (sym ws) = mdl (phy ws) \<and> e_vld env (sym ws) \<and> e_rows (sym ws) = matrices_MyMatrix.rows (mdl (phy ws)) \<and> e_cols (sym ws) = cols (mdl (phy ws))" for env ws
theorem sub'vc:
  fixes a :: "int matrix"
  fixes b :: "int matrix"
  assumes fact0: "infix_eqeqeq (mdl a) (mdl b)"
  shows "let o1 :: int = columns a; o2 :: int = matrix_Matrix.rows a in ((0 :: int) \<le> o2 \<and> (0 :: int) \<le> o1) \<and> (\<forall>(res :: int matrix). matrix_Matrix.rows res = o2 \<and> columns res = o1 \<and> (\<forall>(i :: int) (j :: int). ((0 :: int) \<le> i \<and> i < o2) \<and> (0 :: int) \<le> j \<and> j < o1 \<longrightarrow> elts res i j = (0 :: int)) \<longrightarrow> (let o3 :: int = matrix_Matrix.rows a - (1 :: int) in ((0 :: int) \<le> o3 + (1 :: int) \<longrightarrow> (\<forall>(i' :: int) (j' :: int). (0 :: int) \<le> i' \<and> i' < (0 :: int) \<longrightarrow> (0 :: int) \<le> j' \<and> j' < columns a \<longrightarrow> elts res i' j' = elts a i' j' - elts b i' j') \<and> (\<forall>(res1 :: int matrix). matrix_Matrix.rows res1 = matrix_Matrix.rows res \<and> columns res1 = columns res \<longrightarrow> (\<forall>(i :: int). ((0 :: int) \<le> i \<and> i \<le> o3) \<and> (\<forall>(i' :: int) (j' :: int). (0 :: int) \<le> i' \<and> i' < i \<longrightarrow> (0 :: int) \<le> j' \<and> j' < columns a \<longrightarrow> elts res1 i' j' = elts a i' j' - elts b i' j') \<longrightarrow> (let o4 :: int = columns a - (1 :: int) in ((0 :: int) \<le> o4 + (1 :: int) \<longrightarrow> (\<forall>(j' :: int). (0 :: int) \<le> j' \<and> j' < (0 :: int) \<longrightarrow> elts res1 i j' = elts a i j' - elts b i j') \<and> (\<forall>(res2 :: int matrix). matrix_Matrix.rows res2 = matrix_Matrix.rows res1 \<and> columns res2 = columns res1 \<longrightarrow> (\<forall>(j :: int). ((0 :: int) \<le> j \<and> j \<le> o4) \<and> (\<forall>(i' :: int) (j' :: int). (0 :: int) \<le> i' \<and> i' < i \<longrightarrow> (0 :: int) \<le> j' \<and> j' < columns a \<longrightarrow> elts res2 i' j' = elts res1 i' j') \<and> (\<forall>(j' :: int). (0 :: int) \<le> j' \<and> j' < j \<longrightarrow> elts res2 i j' = elts a i j' - elts b i j') \<longrightarrow> valid_index b i j \<and> valid_index a i j \<and> valid_index res2 i j \<and> (\<forall>(res3 :: int matrix). matrix_Matrix.rows res3 = matrix_Matrix.rows res2 \<and> columns res3 = columns res2 \<longrightarrow> elts res3 = (elts res2)(i := (elts res2 i)(j := elts a i j - elts b i j)) \<longrightarrow> (\<forall>(i' :: int) (j' :: int). (0 :: int) \<le> i' \<and> i' < i \<longrightarrow> (0 :: int) \<le> j' \<and> j' < columns a \<longrightarrow> elts res3 i' j' = elts res1 i' j') \<and> (\<forall>(j' :: int). (0 :: int) \<le> j' \<and> j' < j + (1 :: int) \<longrightarrow> elts res3 i j' = elts a i j' - elts b i j'))) \<and> ((\<forall>(i' :: int) (j' :: int). (0 :: int) \<le> i' \<and> i' < i \<longrightarrow> (0 :: int) \<le> j' \<and> j' < columns a \<longrightarrow> elts res2 i' j' = elts res1 i' j') \<and> (\<forall>(j' :: int). (0 :: int) \<le> j' \<and> j' < o4 + (1 :: int) \<longrightarrow> elts res2 i j' = elts a i j' - elts b i j') \<longrightarrow> (\<forall>(i' :: int) (j' :: int). (0 :: int) \<le> i' \<and> i' < i + (1 :: int) \<longrightarrow> (0 :: int) \<le> j' \<and> j' < columns a \<longrightarrow> elts res2 i' j' = elts a i' j' - elts b i' j')))) \<and> (o4 + (1 :: int) < (0 :: int) \<longrightarrow> (\<forall>(i' :: int) (j' :: int). (0 :: int) \<le> i' \<and> i' < i + (1 :: int) \<longrightarrow> (0 :: int) \<le> j' \<and> j' < columns a \<longrightarrow> elts res1 i' j' = elts a i' j' - elts b i' j')))) \<and> ((\<forall>(i' :: int) (j' :: int). (0 :: int) \<le> i' \<and> i' < o3 + (1 :: int) \<longrightarrow> (0 :: int) \<le> j' \<and> j' < columns a \<longrightarrow> elts res1 i' j' = elts a i' j' - elts b i' j') \<longrightarrow> mdl res1 = sub (mdl a) (mdl b) \<and> infix_eqeqeq (mdl res1) (mdl a)))) \<and> (o3 + (1 :: int) < (0 :: int) \<longrightarrow> mdl res = sub (mdl a) (mdl b) \<and> infix_eqeqeq (mdl res) (mdl a))))"
  sorry
end
