theory string_base64_encoding_Base64_int2b64qtvc
  imports "NTP4Verif.NTP4Verif" "Why3STD.string_StringBuffer"
begin
definition int2b64 :: "int \<Rightarrow> char"
  where "int2b64 i = (if (0 :: int) \<le> i \<and> i \<le> (25 :: int) then char_of (i + (65 :: int)) else if (26 :: int) \<le> i \<and> i \<le> (51 :: int) then char_of (i - (26 :: int) + (97 :: int)) else if (52 :: int) \<le> i \<and> i \<le> (61 :: int) then char_of (i - (52 :: int) + (48 :: int)) else if i = (62 :: int) then char_of (43 :: int) else if i = (63 :: int) then char_of (47 :: int) else char_of (0 :: int))" for i
theorem int2b64'vc:
  fixes i :: "63 word"
  fixes o1 :: "bool"
  assumes fact0: "(0 :: int) \<le> sint i"
  assumes fact1: "sint i < (64 :: int)"
  assumes fact2: "if (0 :: int) \<le> sint i then o1 = (if sint i \<le> (25 :: int) then True else False) else o1 = False"
  shows "if o1 = True then int'63_in_bounds (sint i + (65 :: int)) \<and> (\<forall>(o2 :: 63 word). sint o2 = sint i + (65 :: int) \<longrightarrow> (0 :: int) \<le> sint o2 \<and> sint o2 < (256 :: int)) else \<forall>(o2 :: bool). (if (26 :: int) \<le> sint i then o2 = (if sint i \<le> (51 :: int) then True else False) else o2 = False) \<longrightarrow> (if o2 = True then int'63_in_bounds (sint i - (26 :: int)) \<and> (\<forall>(o3 :: 63 word). sint o3 = sint i - (26 :: int) \<longrightarrow> int'63_in_bounds (sint o3 + (97 :: int)) \<and> (\<forall>(o4 :: 63 word). sint o4 = sint o3 + (97 :: int) \<longrightarrow> (0 :: int) \<le> sint o4 \<and> sint o4 < (256 :: int))) else \<forall>(o3 :: bool). (if (52 :: int) \<le> sint i then o3 = (if sint i \<le> (61 :: int) then True else False) else o3 = False) \<longrightarrow> (if o3 = True then int'63_in_bounds (sint i - (52 :: int)) \<and> (\<forall>(o4 :: 63 word). sint o4 = sint i - (52 :: int) \<longrightarrow> int'63_in_bounds (sint o4 + (48 :: int)) \<and> (\<forall>(o5 :: 63 word). sint o5 = sint o4 + (48 :: int) \<longrightarrow> (0 :: int) \<le> sint o5 \<and> sint o5 < (256 :: int))) else (sint i = (62 :: int) \<longrightarrow> i = (62 :: 63 word)) \<longrightarrow> (if i = (62 :: 63 word) then (0 :: int) \<le> (43 :: int) \<and> (43 :: int) < (256 :: int) else (sint i = (63 :: int) \<longrightarrow> i = (63 :: 63 word)) \<longrightarrow> i = (63 :: 63 word) \<and> (0 :: int) \<le> (47 :: int) \<and> (47 :: int) < (256 :: int))))"
  and "\<forall>(result :: char). (if o1 = True then \<exists>(o2 :: 63 word). sint o2 = sint i + (65 :: int) \<and> result = char_of (sint o2) else \<exists>(o2 :: bool). (if (26 :: int) \<le> sint i then o2 = (if sint i \<le> (51 :: int) then True else False) else o2 = False) \<and> (if o2 = True then \<exists>(o3 :: 63 word). sint o3 = sint i - (26 :: int) \<and> (\<exists>(o4 :: 63 word). sint o4 = sint o3 + (97 :: int) \<and> result = char_of (sint o4)) else \<exists>(o3 :: bool). (if (52 :: int) \<le> sint i then o3 = (if sint i \<le> (61 :: int) then True else False) else o3 = False) \<and> (if o3 = True then \<exists>(o4 :: 63 word). sint o4 = sint i - (52 :: int) \<and> (\<exists>(o5 :: 63 word). sint o5 = sint o4 + (48 :: int) \<and> result = char_of (sint o5)) else (sint i = (62 :: int) \<longrightarrow> i = (62 :: 63 word)) \<and> (if i = (62 :: 63 word) then result = char_of (43 :: int) else (sint i = (63 :: int) \<longrightarrow> i = (63 :: 63 word)) \<and> i = (63 :: 63 word) \<and> result = char_of (47 :: int))))) \<longrightarrow> result = int2b64 (sint i)"
  sorry
end
