theory array_of_list_Top_array_of_listqtvc
  imports "NTP4Verif.NTP4Verif"
begin
theorem array_of_list'vc:
  fixes l :: "'a list"
  fixes o1 :: "nat"
  fixes n :: "63 word"
  assumes fact0: "\<not>l = (Nil :: 'a list)"
  assumes fact1: "o1 = length l"
  assumes fact2: "sint n = int o1"
  shows "case l of (Nil :: 'a list) \<Rightarrow> False | Cons x ll \<Rightarrow> (0 :: int) \<le> sint n \<and> (\<forall>(a :: 'a array63). (\<forall>(i :: int). (0 :: int) \<le> i \<and> i < sint n \<longrightarrow> array63_elts a ! nat i = x) \<and> array63_length a = n \<longrightarrow> (\<forall>(a1 :: 'a array63). array63_length a1 = array63_length a \<longrightarrow> (\<forall>(i :: 63 word) (ll1 :: 'a list). ((1 :: int) \<le> sint i \<and> sint n - sint i = int (length ll1)) \<and> (\<forall>(j :: int). (0 :: int) \<le> j \<and> j < sint i \<longrightarrow> Some (array63_elts a1 ! nat j) = nth_opt l j) \<and> (\<forall>(j :: int). sint i \<le> j \<and> j < sint n \<longrightarrow> nth_opt ll1 (j - sint i) = nth_opt l j) \<longrightarrow> (case ll1 of (Nil :: 'a list) \<Rightarrow> (\<forall>(j :: int). (0 :: int) \<le> j \<and> j < sint n \<longrightarrow> Some (array63_elts a1 ! nat j) = nth_opt l j) | Cons x1 ll2 \<Rightarrow> ((0 :: int) \<le> sint i \<and> sint i < sint (array63_length a1)) \<and> (\<forall>(a2 :: 'a array63). array63_length a2 = array63_length a1 \<longrightarrow> array63_elts a2 = (array63_elts a1)[nat (sint i) := x1] \<longrightarrow> int'63_in_bounds (sint i + (1 :: int)) \<and> (\<forall>(o2 :: 63 word). sint o2 = sint i + (1 :: int) \<longrightarrow> ((0 :: int) \<le> sint n - sint i \<and> sint n - sint o2 < sint n - sint i) \<and> ((1 :: int) \<le> sint o2 \<and> sint n - sint o2 = int (length ll2)) \<and> (\<forall>(j :: int). (0 :: int) \<le> j \<and> j < sint o2 \<longrightarrow> Some (array63_elts a2 ! nat j) = nth_opt l j) \<and> (\<forall>(j :: int). sint o2 \<le> j \<and> j < sint n \<longrightarrow> nth_opt ll2 (j - sint o2) = nth_opt l j)))))) \<and> (((1 :: int) \<le> (1 :: int) \<and> sint n - (1 :: int) = int (length ll)) \<and> (\<forall>(j :: int). (0 :: int) \<le> j \<and> j < (1 :: int) \<longrightarrow> Some (array63_elts a ! nat j) = nth_opt l j) \<and> (\<forall>(j :: int). (1 :: int) \<le> j \<and> j < sint n \<longrightarrow> nth_opt ll (j - (1 :: int)) = nth_opt l j)) \<and> (\<forall>(a1 :: 'a array63). array63_length a1 = array63_length a \<longrightarrow> (\<forall>(j :: int). (0 :: int) \<le> j \<and> j < sint n \<longrightarrow> Some (array63_elts a1 ! nat j) = nth_opt l j) \<longrightarrow> sint (array63_length a1) = int (length l) \<and> (\<forall>(i :: int). (0 :: int) \<le> i \<and> i < int (length l) \<longrightarrow> Some (array63_elts a1 ! nat i) = nth_opt l i)))"
  sorry
end
