theory verifythis_2017_pair_insertion_sort_Challenge1_pair_insertion_sortqtvc
  imports "NTP4Verif.NTP4Verif" "Why3STD.Ref_Ref" "Why3STD.map_MapEq" "Why3STD.map_MapExchange" "Why3STD.map_MapPermut"
begin
theorem pair_insertion_sort'vc:
  fixes a :: "int list"
  shows "(0 :: int) \<le> (0 :: int)"
  and "(0 :: int) \<le> int (length a)"
  and "\<forall>(k :: int) (l :: int). (0 :: int) \<le> k \<and> k \<le> l \<and> l < (0 :: int) \<longrightarrow> a ! nat k \<le> a ! nat l"
  and "a <~~> a"
  and "\<forall>(i :: int) (a1 :: int list). length a1 = length a \<longrightarrow> ((0 :: int) \<le> i \<and> i \<le> int (length a1)) \<and> (\<forall>(k :: int) (l :: int). (0 :: int) \<le> k \<and> k \<le> l \<and> l < i \<longrightarrow> a1 ! nat k \<le> a1 ! nat l) \<and> a <~~> a1 \<longrightarrow> (if i < int (length a1) - (1 :: int) then ((0 :: int) \<le> i \<and> i < int (length a1)) \<and> (let o1 :: int = a1 ! nat i; o2 :: int = i + (1 :: int) in ((0 :: int) \<le> o2 \<and> o2 < int (length a1)) \<and> (let o3 :: int = a1 ! nat o2 in if o1 < o3 then let o4 :: int = i - (1 :: int) in ((-(1 :: int) \<le> o4 \<and> o4 < i) \<and> (\<forall>(k :: int) (l :: int). (0 :: int) \<le> k \<and> k \<le> l \<and> l \<le> o4 \<longrightarrow> a1 ! nat k \<le> a1 ! nat l) \<and> (\<forall>(k :: int) (l :: int). (0 :: int) \<le> k \<and> k \<le> o4 \<longrightarrow> o4 + (2 :: int) < l \<and> l < i + (2 :: int) \<longrightarrow> a1 ! nat k \<le> a1 ! nat l) \<and> (\<forall>(k :: int) (l :: int). o4 + (2 :: int) < k \<and> k \<le> l \<and> l < i + (2 :: int) \<longrightarrow> a1 ! nat k \<le> a1 ! nat l) \<and> (\<forall>(l :: int). o4 + (2 :: int) < l \<and> l < i + (2 :: int) \<longrightarrow> o3 < a1 ! nat l) \<and> a <~~> a1[nat (o4 + (2 :: int)) := o3, nat (o4 + (1 :: int)) := o1]) \<and> (\<forall>(j :: int) (a2 :: int list). length a2 = length a1 \<longrightarrow> (-(1 :: int) \<le> j \<and> j < i) \<and> (\<forall>(k :: int) (l :: int). (0 :: int) \<le> k \<and> k \<le> l \<and> l \<le> j \<longrightarrow> a2 ! nat k \<le> a2 ! nat l) \<and> (\<forall>(k :: int) (l :: int). (0 :: int) \<le> k \<and> k \<le> j \<longrightarrow> j + (2 :: int) < l \<and> l < i + (2 :: int) \<longrightarrow> a2 ! nat k \<le> a2 ! nat l) \<and> (\<forall>(k :: int) (l :: int). j + (2 :: int) < k \<and> k \<le> l \<and> l < i + (2 :: int) \<longrightarrow> a2 ! nat k \<le> a2 ! nat l) \<and> (\<forall>(l :: int). j + (2 :: int) < l \<and> l < i + (2 :: int) \<longrightarrow> o3 < a2 ! nat l) \<and> a <~~> a2[nat (j + (2 :: int)) := o3, nat (j + (1 :: int)) := o1] \<longrightarrow> ((0 :: int) \<le> j \<longrightarrow> (0 :: int) \<le> j \<and> j < int (length a2)) \<and> (\<forall>(o5 :: bool). (if (0 :: int) \<le> j then o5 = (if o3 < a2 ! nat j then True else False) else o5 = False) \<longrightarrow> (if o5 = True then ((0 :: int) \<le> j \<and> j < int (length a2)) \<and> (let o6 :: int = a2 ! nat j; o7 :: int = j + (2 :: int) in ((0 :: int) \<le> o7 \<and> o7 < int (length a2)) \<and> (length (a2[nat o7 := o6]) = length a2 \<longrightarrow> nth (a2[nat o7 := o6]) o nat = (nth a2 o nat)(o7 := o6) \<longrightarrow> ((0 :: int) \<le> j \<and> j - (1 :: int) < j) \<and> (-(1 :: int) \<le> j - (1 :: int) \<and> j - (1 :: int) < i) \<and> (\<forall>(k :: int) (l :: int). (0 :: int) \<le> k \<and> k \<le> l \<and> l \<le> j - (1 :: int) \<longrightarrow> a2[nat o7 := o6] ! nat k \<le> a2[nat o7 := o6] ! nat l) \<and> (\<forall>(k :: int) (l :: int). (0 :: int) \<le> k \<and> k \<le> j - (1 :: int) \<longrightarrow> j - (1 :: int) + (2 :: int) < l \<and> l < i + (2 :: int) \<longrightarrow> a2[nat o7 := o6] ! nat k \<le> a2[nat o7 := o6] ! nat l) \<and> (\<forall>(k :: int) (l :: int). j - (1 :: int) + (2 :: int) < k \<and> k \<le> l \<and> l < i + (2 :: int) \<longrightarrow> a2[nat o7 := o6] ! nat k \<le> a2[nat o7 := o6] ! nat l) \<and> (\<forall>(l :: int). j - (1 :: int) + (2 :: int) < l \<and> l < i + (2 :: int) \<longrightarrow> o3 < a2[nat o7 := o6] ! nat l) \<and> a <~~> a2[nat (j - (1 :: int) + (2 :: int)) := o3, nat (j - (1 :: int) + (1 :: int)) := o1, nat o7 := o6])) else let o6 :: int = j + (2 :: int) in ((0 :: int) \<le> o6 \<and> o6 < int (length a2)) \<and> (length (a2[nat o6 := o3]) = length a2 \<longrightarrow> nth (a2[nat o6 := o3]) o nat = (nth a2 o nat)(o6 := o3) \<longrightarrow> ((-(1 :: int) \<le> j \<and> j < i) \<and> (\<forall>(k :: int) (l :: int). (0 :: int) \<le> k \<and> k \<le> l \<and> l \<le> j \<longrightarrow> a2[nat o6 := o3] ! nat k \<le> a2[nat o6 := o3] ! nat l) \<and> (\<forall>(k :: int) (l :: int). (0 :: int) \<le> k \<and> k \<le> j \<longrightarrow> j + (1 :: int) < l \<and> l < i + (2 :: int) \<longrightarrow> a2[nat o6 := o3] ! nat k \<le> a2[nat o6 := o3] ! nat l) \<and> (\<forall>(k :: int) (l :: int). j + (1 :: int) < k \<and> k \<le> l \<and> l < i + (2 :: int) \<longrightarrow> a2[nat o6 := o3] ! nat k \<le> a2[nat o6 := o3] ! nat l) \<and> (\<forall>(l :: int). j + (1 :: int) < l \<and> l < i + (2 :: int) \<longrightarrow> o1 \<le> a2[nat o6 := o3] ! nat l) \<and> a <~~> a2[nat (j + (1 :: int)) := o1, nat o6 := o3]) \<and> (\<forall>(j1 :: int) (a3 :: int list). length a3 = length (a2[nat o6 := o3]) \<longrightarrow> (-(1 :: int) \<le> j1 \<and> j1 < i) \<and> (\<forall>(k :: int) (l :: int). (0 :: int) \<le> k \<and> k \<le> l \<and> l \<le> j1 \<longrightarrow> a3 ! nat k \<le> a3 ! nat l) \<and> (\<forall>(k :: int) (l :: int). (0 :: int) \<le> k \<and> k \<le> j1 \<longrightarrow> j1 + (1 :: int) < l \<and> l < i + (2 :: int) \<longrightarrow> a3 ! nat k \<le> a3 ! nat l) \<and> (\<forall>(k :: int) (l :: int). j1 + (1 :: int) < k \<and> k \<le> l \<and> l < i + (2 :: int) \<longrightarrow> a3 ! nat k \<le> a3 ! nat l) \<and> (\<forall>(l :: int). j1 + (1 :: int) < l \<and> l < i + (2 :: int) \<longrightarrow> o1 \<le> a3 ! nat l) \<and> a <~~> a3[nat (j1 + (1 :: int)) := o1] \<longrightarrow> ((0 :: int) \<le> j1 \<longrightarrow> (0 :: int) \<le> j1 \<and> j1 < int (length a3)) \<and> (\<forall>(o7 :: bool). (if (0 :: int) \<le> j1 then o7 = (if o1 < a3 ! nat j1 then True else False) else o7 = False) \<longrightarrow> (if o7 = True then ((0 :: int) \<le> j1 \<and> j1 < int (length a3)) \<and> (let o8 :: int = a3 ! nat j1; o9 :: int = j1 + (1 :: int) in ((0 :: int) \<le> o9 \<and> o9 < int (length a3)) \<and> (length (a3[nat o9 := o8]) = length a3 \<longrightarrow> nth (a3[nat o9 := o8]) o nat = (nth a3 o nat)(o9 := o8) \<longrightarrow> ((0 :: int) \<le> j1 \<and> j1 - (1 :: int) < j1) \<and> (-(1 :: int) \<le> j1 - (1 :: int) \<and> j1 - (1 :: int) < i) \<and> (\<forall>(k :: int) (l :: int). (0 :: int) \<le> k \<and> k \<le> l \<and> l \<le> j1 - (1 :: int) \<longrightarrow> a3[nat o9 := o8] ! nat k \<le> a3[nat o9 := o8] ! nat l) \<and> (\<forall>(k :: int) (l :: int). (0 :: int) \<le> k \<and> k \<le> j1 - (1 :: int) \<longrightarrow> j1 - (1 :: int) + (1 :: int) < l \<and> l < i + (2 :: int) \<longrightarrow> a3[nat o9 := o8] ! nat k \<le> a3[nat o9 := o8] ! nat l) \<and> (\<forall>(k :: int) (l :: int). j1 - (1 :: int) + (1 :: int) < k \<and> k \<le> l \<and> l < i + (2 :: int) \<longrightarrow> a3[nat o9 := o8] ! nat k \<le> a3[nat o9 := o8] ! nat l) \<and> (\<forall>(l :: int). j1 - (1 :: int) + (1 :: int) < l \<and> l < i + (2 :: int) \<longrightarrow> o1 \<le> a3[nat o9 := o8] ! nat l) \<and> a <~~> a3[nat (j1 - (1 :: int) + (1 :: int)) := o1, nat o9 := o8])) else let o8 :: int = j1 + (1 :: int) in ((0 :: int) \<le> o8 \<and> o8 < int (length a3)) \<and> (length (a3[nat o8 := o1]) = length a3 \<longrightarrow> nth (a3[nat o8 := o1]) o nat = (nth a3 o nat)(o8 := o1) \<longrightarrow> ((0 :: int) \<le> int (length a1) - i \<and> int (length (a3[nat o8 := o1])) - (i + (2 :: int)) < int (length a1) - i) \<and> ((0 :: int) \<le> i + (2 :: int) \<and> i + (2 :: int) \<le> int (length (a3[nat o8 := o1]))) \<and> (\<forall>(k :: int) (l :: int). (0 :: int) \<le> k \<and> k \<le> l \<and> l < i + (2 :: int) \<longrightarrow> a3[nat o8 := o1] ! nat k \<le> a3[nat o8 := o1] ! nat l) \<and> a <~~> a3[nat o8 := o1])))))))) else let o4 :: int = i - (1 :: int) in ((-(1 :: int) \<le> o4 \<and> o4 < i) \<and> (\<forall>(k :: int) (l :: int). (0 :: int) \<le> k \<and> k \<le> l \<and> l \<le> o4 \<longrightarrow> a1 ! nat k \<le> a1 ! nat l) \<and> (\<forall>(k :: int) (l :: int). (0 :: int) \<le> k \<and> k \<le> o4 \<longrightarrow> o4 + (2 :: int) < l \<and> l < i + (2 :: int) \<longrightarrow> a1 ! nat k \<le> a1 ! nat l) \<and> (\<forall>(k :: int) (l :: int). o4 + (2 :: int) < k \<and> k \<le> l \<and> l < i + (2 :: int) \<longrightarrow> a1 ! nat k \<le> a1 ! nat l) \<and> (\<forall>(l :: int). o4 + (2 :: int) < l \<and> l < i + (2 :: int) \<longrightarrow> o1 < a1 ! nat l) \<and> a <~~> a1[nat (o4 + (2 :: int)) := o1, nat (o4 + (1 :: int)) := o3]) \<and> (\<forall>(j :: int) (a2 :: int list). length a2 = length a1 \<longrightarrow> (-(1 :: int) \<le> j \<and> j < i) \<and> (\<forall>(k :: int) (l :: int). (0 :: int) \<le> k \<and> k \<le> l \<and> l \<le> j \<longrightarrow> a2 ! nat k \<le> a2 ! nat l) \<and> (\<forall>(k :: int) (l :: int). (0 :: int) \<le> k \<and> k \<le> j \<longrightarrow> j + (2 :: int) < l \<and> l < i + (2 :: int) \<longrightarrow> a2 ! nat k \<le> a2 ! nat l) \<and> (\<forall>(k :: int) (l :: int). j + (2 :: int) < k \<and> k \<le> l \<and> l < i + (2 :: int) \<longrightarrow> a2 ! nat k \<le> a2 ! nat l) \<and> (\<forall>(l :: int). j + (2 :: int) < l \<and> l < i + (2 :: int) \<longrightarrow> o1 < a2 ! nat l) \<and> a <~~> a2[nat (j + (2 :: int)) := o1, nat (j + (1 :: int)) := o3] \<longrightarrow> ((0 :: int) \<le> j \<longrightarrow> (0 :: int) \<le> j \<and> j < int (length a2)) \<and> (\<forall>(o5 :: bool). (if (0 :: int) \<le> j then o5 = (if o1 < a2 ! nat j then True else False) else o5 = False) \<longrightarrow> (if o5 = True then ((0 :: int) \<le> j \<and> j < int (length a2)) \<and> (let o6 :: int = a2 ! nat j; o7 :: int = j + (2 :: int) in ((0 :: int) \<le> o7 \<and> o7 < int (length a2)) \<and> (length (a2[nat o7 := o6]) = length a2 \<longrightarrow> nth (a2[nat o7 := o6]) o nat = (nth a2 o nat)(o7 := o6) \<longrightarrow> ((0 :: int) \<le> j \<and> j - (1 :: int) < j) \<and> (-(1 :: int) \<le> j - (1 :: int) \<and> j - (1 :: int) < i) \<and> (\<forall>(k :: int) (l :: int). (0 :: int) \<le> k \<and> k \<le> l \<and> l \<le> j - (1 :: int) \<longrightarrow> a2[nat o7 := o6] ! nat k \<le> a2[nat o7 := o6] ! nat l) \<and> (\<forall>(k :: int) (l :: int). (0 :: int) \<le> k \<and> k \<le> j - (1 :: int) \<longrightarrow> j - (1 :: int) + (2 :: int) < l \<and> l < i + (2 :: int) \<longrightarrow> a2[nat o7 := o6] ! nat k \<le> a2[nat o7 := o6] ! nat l) \<and> (\<forall>(k :: int) (l :: int). j - (1 :: int) + (2 :: int) < k \<and> k \<le> l \<and> l < i + (2 :: int) \<longrightarrow> a2[nat o7 := o6] ! nat k \<le> a2[nat o7 := o6] ! nat l) \<and> (\<forall>(l :: int). j - (1 :: int) + (2 :: int) < l \<and> l < i + (2 :: int) \<longrightarrow> o1 < a2[nat o7 := o6] ! nat l) \<and> a <~~> a2[nat (j - (1 :: int) + (2 :: int)) := o1, nat (j - (1 :: int) + (1 :: int)) := o3, nat o7 := o6])) else let o6 :: int = j + (2 :: int) in ((0 :: int) \<le> o6 \<and> o6 < int (length a2)) \<and> (length (a2[nat o6 := o1]) = length a2 \<longrightarrow> nth (a2[nat o6 := o1]) o nat = (nth a2 o nat)(o6 := o1) \<longrightarrow> ((-(1 :: int) \<le> j \<and> j < i) \<and> (\<forall>(k :: int) (l :: int). (0 :: int) \<le> k \<and> k \<le> l \<and> l \<le> j \<longrightarrow> a2[nat o6 := o1] ! nat k \<le> a2[nat o6 := o1] ! nat l) \<and> (\<forall>(k :: int) (l :: int). (0 :: int) \<le> k \<and> k \<le> j \<longrightarrow> j + (1 :: int) < l \<and> l < i + (2 :: int) \<longrightarrow> a2[nat o6 := o1] ! nat k \<le> a2[nat o6 := o1] ! nat l) \<and> (\<forall>(k :: int) (l :: int). j + (1 :: int) < k \<and> k \<le> l \<and> l < i + (2 :: int) \<longrightarrow> a2[nat o6 := o1] ! nat k \<le> a2[nat o6 := o1] ! nat l) \<and> (\<forall>(l :: int). j + (1 :: int) < l \<and> l < i + (2 :: int) \<longrightarrow> o3 \<le> a2[nat o6 := o1] ! nat l) \<and> a <~~> a2[nat (j + (1 :: int)) := o3, nat o6 := o1]) \<and> (\<forall>(j1 :: int) (a3 :: int list). length a3 = length (a2[nat o6 := o1]) \<longrightarrow> (-(1 :: int) \<le> j1 \<and> j1 < i) \<and> (\<forall>(k :: int) (l :: int). (0 :: int) \<le> k \<and> k \<le> l \<and> l \<le> j1 \<longrightarrow> a3 ! nat k \<le> a3 ! nat l) \<and> (\<forall>(k :: int) (l :: int). (0 :: int) \<le> k \<and> k \<le> j1 \<longrightarrow> j1 + (1 :: int) < l \<and> l < i + (2 :: int) \<longrightarrow> a3 ! nat k \<le> a3 ! nat l) \<and> (\<forall>(k :: int) (l :: int). j1 + (1 :: int) < k \<and> k \<le> l \<and> l < i + (2 :: int) \<longrightarrow> a3 ! nat k \<le> a3 ! nat l) \<and> (\<forall>(l :: int). j1 + (1 :: int) < l \<and> l < i + (2 :: int) \<longrightarrow> o3 \<le> a3 ! nat l) \<and> a <~~> a3[nat (j1 + (1 :: int)) := o3] \<longrightarrow> ((0 :: int) \<le> j1 \<longrightarrow> (0 :: int) \<le> j1 \<and> j1 < int (length a3)) \<and> (\<forall>(o7 :: bool). (if (0 :: int) \<le> j1 then o7 = (if o3 < a3 ! nat j1 then True else False) else o7 = False) \<longrightarrow> (if o7 = True then ((0 :: int) \<le> j1 \<and> j1 < int (length a3)) \<and> (let o8 :: int = a3 ! nat j1; o9 :: int = j1 + (1 :: int) in ((0 :: int) \<le> o9 \<and> o9 < int (length a3)) \<and> (length (a3[nat o9 := o8]) = length a3 \<longrightarrow> nth (a3[nat o9 := o8]) o nat = (nth a3 o nat)(o9 := o8) \<longrightarrow> ((0 :: int) \<le> j1 \<and> j1 - (1 :: int) < j1) \<and> (-(1 :: int) \<le> j1 - (1 :: int) \<and> j1 - (1 :: int) < i) \<and> (\<forall>(k :: int) (l :: int). (0 :: int) \<le> k \<and> k \<le> l \<and> l \<le> j1 - (1 :: int) \<longrightarrow> a3[nat o9 := o8] ! nat k \<le> a3[nat o9 := o8] ! nat l) \<and> (\<forall>(k :: int) (l :: int). (0 :: int) \<le> k \<and> k \<le> j1 - (1 :: int) \<longrightarrow> j1 - (1 :: int) + (1 :: int) < l \<and> l < i + (2 :: int) \<longrightarrow> a3[nat o9 := o8] ! nat k \<le> a3[nat o9 := o8] ! nat l) \<and> (\<forall>(k :: int) (l :: int). j1 - (1 :: int) + (1 :: int) < k \<and> k \<le> l \<and> l < i + (2 :: int) \<longrightarrow> a3[nat o9 := o8] ! nat k \<le> a3[nat o9 := o8] ! nat l) \<and> (\<forall>(l :: int). j1 - (1 :: int) + (1 :: int) < l \<and> l < i + (2 :: int) \<longrightarrow> o3 \<le> a3[nat o9 := o8] ! nat l) \<and> a <~~> a3[nat (j1 - (1 :: int) + (1 :: int)) := o3, nat o9 := o8])) else let o8 :: int = j1 + (1 :: int) in ((0 :: int) \<le> o8 \<and> o8 < int (length a3)) \<and> (length (a3[nat o8 := o3]) = length a3 \<longrightarrow> nth (a3[nat o8 := o3]) o nat = (nth a3 o nat)(o8 := o3) \<longrightarrow> ((0 :: int) \<le> int (length a1) - i \<and> int (length (a3[nat o8 := o3])) - (i + (2 :: int)) < int (length a1) - i) \<and> ((0 :: int) \<le> i + (2 :: int) \<and> i + (2 :: int) \<le> int (length (a3[nat o8 := o3]))) \<and> (\<forall>(k :: int) (l :: int). (0 :: int) \<le> k \<and> k \<le> l \<and> l < i + (2 :: int) \<longrightarrow> a3[nat o8 := o3] ! nat k \<le> a3[nat o8 := o3] ! nat l) \<and> a <~~> a3[nat o8 := o3])))))))))) else if i = int (length a1) - (1 :: int) then ((0 :: int) \<le> i \<and> i < int (length a1)) \<and> (let y :: int = a1 ! nat i; o1 :: int = i - (1 :: int) in ((-(1 :: int) \<le> o1 \<and> o1 < i) \<and> (\<forall>(k :: int) (l :: int). (0 :: int) \<le> k \<and> k \<le> l \<and> l \<le> o1 \<longrightarrow> a1 ! nat k \<le> a1 ! nat l) \<and> (\<forall>(k :: int) (l :: int). (0 :: int) \<le> k \<and> k \<le> o1 \<longrightarrow> o1 + (1 :: int) < l \<and> l < int (length a1) \<longrightarrow> a1 ! nat k \<le> a1 ! nat l) \<and> (\<forall>(k :: int) (l :: int). o1 + (1 :: int) < k \<and> k \<le> l \<and> l < int (length a1) \<longrightarrow> a1 ! nat k \<le> a1 ! nat l) \<and> (\<forall>(l :: int). o1 + (1 :: int) < l \<and> l < int (length a1) \<longrightarrow> y < a1 ! nat l) \<and> a <~~> a1[nat (o1 + (1 :: int)) := y]) \<and> (\<forall>(j :: int) (a2 :: int list). length a2 = length a1 \<longrightarrow> (-(1 :: int) \<le> j \<and> j < i) \<and> (\<forall>(k :: int) (l :: int). (0 :: int) \<le> k \<and> k \<le> l \<and> l \<le> j \<longrightarrow> a2 ! nat k \<le> a2 ! nat l) \<and> (\<forall>(k :: int) (l :: int). (0 :: int) \<le> k \<and> k \<le> j \<longrightarrow> j + (1 :: int) < l \<and> l < int (length a2) \<longrightarrow> a2 ! nat k \<le> a2 ! nat l) \<and> (\<forall>(k :: int) (l :: int). j + (1 :: int) < k \<and> k \<le> l \<and> l < int (length a2) \<longrightarrow> a2 ! nat k \<le> a2 ! nat l) \<and> (\<forall>(l :: int). j + (1 :: int) < l \<and> l < int (length a2) \<longrightarrow> y < a2 ! nat l) \<and> a <~~> a2[nat (j + (1 :: int)) := y] \<longrightarrow> ((0 :: int) \<le> j \<longrightarrow> (0 :: int) \<le> j \<and> j < int (length a2)) \<and> (\<forall>(o2 :: bool). (if (0 :: int) \<le> j then o2 = (if y < a2 ! nat j then True else False) else o2 = False) \<longrightarrow> (if o2 = True then ((0 :: int) \<le> j \<and> j < int (length a2)) \<and> (let o3 :: int = a2 ! nat j; o4 :: int = j + (1 :: int) in ((0 :: int) \<le> o4 \<and> o4 < int (length a2)) \<and> (length (a2[nat o4 := o3]) = length a2 \<longrightarrow> nth (a2[nat o4 := o3]) o nat = (nth a2 o nat)(o4 := o3) \<longrightarrow> ((0 :: int) \<le> j \<and> j - (1 :: int) < j) \<and> (-(1 :: int) \<le> j - (1 :: int) \<and> j - (1 :: int) < i) \<and> (\<forall>(k :: int) (l :: int). (0 :: int) \<le> k \<and> k \<le> l \<and> l \<le> j - (1 :: int) \<longrightarrow> a2[nat o4 := o3] ! nat k \<le> a2[nat o4 := o3] ! nat l) \<and> (\<forall>(k :: int) (l :: int). (0 :: int) \<le> k \<and> k \<le> j - (1 :: int) \<longrightarrow> j - (1 :: int) + (1 :: int) < l \<and> l < int (length (a2[nat o4 := o3])) \<longrightarrow> a2[nat o4 := o3] ! nat k \<le> a2[nat o4 := o3] ! nat l) \<and> (\<forall>(k :: int) (l :: int). j - (1 :: int) + (1 :: int) < k \<and> k \<le> l \<and> l < int (length (a2[nat o4 := o3])) \<longrightarrow> a2[nat o4 := o3] ! nat k \<le> a2[nat o4 := o3] ! nat l) \<and> (\<forall>(l :: int). j - (1 :: int) + (1 :: int) < l \<and> l < int (length (a2[nat o4 := o3])) \<longrightarrow> y < a2[nat o4 := o3] ! nat l) \<and> a <~~> a2[nat (j - (1 :: int) + (1 :: int)) := y, nat o4 := o3])) else let o3 :: int = j + (1 :: int) in ((0 :: int) \<le> o3 \<and> o3 < int (length a2)) \<and> (length (a2[nat o3 := y]) = length a2 \<longrightarrow> nth (a2[nat o3 := y]) o nat = (nth a2 o nat)(o3 := y) \<longrightarrow> (\<forall>(k :: int) (l :: int). (0 :: int) \<le> k \<and> k \<le> l \<and> l < int (length (a2[nat o3 := y])) \<longrightarrow> a2[nat o3 := y] ! nat k \<le> a2[nat o3 := y] ! nat l) \<and> a <~~> a2[nat o3 := y]))))) else (\<forall>(k :: int) (l :: int). (0 :: int) \<le> k \<and> k \<le> l \<and> l < int (length a1) \<longrightarrow> a1 ! nat k \<le> a1 ! nat l) \<and> a <~~> a1)"
  sorry
end
