theory longest_increasing_subsequence_Backtracking_lissqtvc
  imports "NTP4Verif.NTP4Verif" "Why3STD.Ref_Ref" "./longest_increasing_subsequence_Spec"
begin
theorem liss'vc:
  fixes w :: "elt list"
  shows "\<forall>(i :: int). (0 :: int) \<le> i \<and> i < int (length w) \<longrightarrow> (let o1 :: int list = [i] in int (length o1) = (1 :: int) \<and> o1 ! (0 :: nat) = i \<longrightarrow> (let o2 :: int = int (length w) - (1 :: int); o3 :: int = i + (1 :: int) in (o3 \<le> o2 + (1 :: int) \<longrightarrow> (((1 :: int) = int (length o1) \<and> (0 :: int) < int (length o1)) \<and> o1 ! (0 :: nat) = i \<and> iss o1 w \<and> (\<forall>(s' :: int list). iss s' w \<longrightarrow> (2 :: int) \<le> int (length s') \<longrightarrow> s' ! (0 :: nat) = i \<and> i < s' ! (1 :: nat) \<and> s' ! (1 :: nat) < o3 \<longrightarrow> length s' \<le> length o1)) \<and> (\<forall>(s :: int list) (len :: int). (\<forall>(j :: int). (o3 \<le> j \<and> j \<le> o2) \<and> (len = int (length s) \<and> (0 :: int) < int (length s)) \<and> s ! (0 :: nat) = i \<and> iss s w \<and> (\<forall>(s' :: int list). iss s' w \<longrightarrow> (2 :: int) \<le> int (length s') \<longrightarrow> s' ! (0 :: nat) = i \<and> i < s' ! (1 :: nat) \<and> s' ! (1 :: nat) < j \<longrightarrow> length s' \<le> length s) \<longrightarrow> (if lt (w ! nat i) (w ! nat j) then (((0 :: int) \<le> int (length w) - i \<and> int (length w) - j < int (length w) - i) \<and> (0 :: int) \<le> j \<and> j < int (length w)) \<and> (\<forall>(sj :: int list). (0 :: int) < int (length sj) \<and> sj ! (0 :: nat) = j \<and> iss sj w \<and> (\<forall>(s' :: int list). iss s' w \<longrightarrow> (1 :: int) \<le> int (length s') \<longrightarrow> s' ! (0 :: nat) = j \<longrightarrow> length s' \<le> length sj) \<longrightarrow> (if len < (1 :: int) + int (length sj) then let o4 :: int list = Cons i sj in int (length o4) = (1 :: int) + int (length sj) \<and> o4 ! (0 :: nat) = i \<and> (\<forall>(i1 :: int). (0 :: int) < i1 \<and> i1 \<le> int (length sj) \<longrightarrow> o4 ! nat i1 = sj ! nat (i1 - (1 :: int))) \<longrightarrow> ((1 :: int) + int (length sj) = int (length o4) \<and> (0 :: int) < int (length o4)) \<and> o4 ! (0 :: nat) = i \<and> iss o4 w \<and> (\<forall>(s' :: int list). iss s' w \<longrightarrow> (2 :: int) \<le> int (length s') \<longrightarrow> s' ! (0 :: nat) = i \<and> i < s' ! (1 :: nat) \<and> s' ! (1 :: nat) < j + (1 :: int) \<longrightarrow> length s' \<le> length o4) else (len = int (length s) \<and> (0 :: int) < int (length s)) \<and> s ! (0 :: nat) = i \<and> iss s w \<and> (\<forall>(s' :: int list). iss s' w \<longrightarrow> (2 :: int) \<le> int (length s') \<longrightarrow> s' ! (0 :: nat) = i \<and> i < s' ! (1 :: nat) \<and> s' ! (1 :: nat) < j + (1 :: int) \<longrightarrow> length s' \<le> length s))) else (len = int (length s) \<and> (0 :: int) < int (length s)) \<and> s ! (0 :: nat) = i \<and> iss s w \<and> (\<forall>(s' :: int list). iss s' w \<longrightarrow> (2 :: int) \<le> int (length s') \<longrightarrow> s' ! (0 :: nat) = i \<and> i < s' ! (1 :: nat) \<and> s' ! (1 :: nat) < j + (1 :: int) \<longrightarrow> length s' \<le> length s))) \<and> ((len = int (length s) \<and> (0 :: int) < int (length s)) \<and> s ! (0 :: nat) = i \<and> iss s w \<and> (\<forall>(s' :: int list). iss s' w \<longrightarrow> (2 :: int) \<le> int (length s') \<longrightarrow> s' ! (0 :: nat) = i \<and> i < s' ! (1 :: nat) \<and> s' ! (1 :: nat) < o2 + (1 :: int) \<longrightarrow> length s' \<le> length s) \<longrightarrow> (len = int (length s) \<and> (0 :: int) < int (length s)) \<and> s ! (0 :: nat) = i \<and> iss s w \<and> (\<forall>(s' :: int list). iss s' w \<longrightarrow> (1 :: int) \<le> int (length s') \<longrightarrow> s' ! (0 :: nat) = i \<longrightarrow> length s' \<le> length s)))) \<and> (o2 + (1 :: int) < o3 \<longrightarrow> ((1 :: int) = int (length o1) \<and> (0 :: int) < int (length o1)) \<and> o1 ! (0 :: nat) = i \<and> iss o1 w \<and> (\<forall>(s' :: int list). iss s' w \<longrightarrow> (1 :: int) \<le> int (length s') \<longrightarrow> s' ! (0 :: nat) = i \<longrightarrow> length s' \<le> length o1))))"
  and "let o1 :: int = int (length w) - (1 :: int) in ((0 :: int) \<le> o1 + (1 :: int) \<longrightarrow> ((0 :: int) = int (length []) \<and> iss [] w \<and> (\<forall>(s' :: int list). iss s' w \<longrightarrow> (1 :: int) \<le> int (length s') \<longrightarrow> s' ! (0 :: nat) < (0 :: int) \<longrightarrow> length s' \<le> length [])) \<and> (\<forall>(s :: int list) (len :: int). (\<forall>(i :: int). ((0 :: int) \<le> i \<and> i \<le> o1) \<and> len = int (length s) \<and> iss s w \<and> (\<forall>(s' :: int list). iss s' w \<longrightarrow> (1 :: int) \<le> int (length s') \<longrightarrow> s' ! (0 :: nat) < i \<longrightarrow> length s' \<le> length s) \<longrightarrow> ((0 :: int) \<le> i \<and> i < int (length w)) \<and> (\<forall>(si :: int list). (0 :: int) < int (length si) \<and> si ! (0 :: nat) = i \<and> iss si w \<and> (\<forall>(s' :: int list). iss s' w \<longrightarrow> (1 :: int) \<le> int (length s') \<longrightarrow> s' ! (0 :: nat) = i \<longrightarrow> length s' \<le> length si) \<longrightarrow> (if len < int (length si) then iss si w \<and> (\<forall>(s' :: int list). iss s' w \<longrightarrow> (1 :: int) \<le> int (length s') \<longrightarrow> s' ! (0 :: nat) < i + (1 :: int) \<longrightarrow> length s' \<le> length si) else len = int (length s) \<and> iss s w \<and> (\<forall>(s' :: int list). iss s' w \<longrightarrow> (1 :: int) \<le> int (length s') \<longrightarrow> s' ! (0 :: nat) < i + (1 :: int) \<longrightarrow> length s' \<le> length s)))) \<and> (len = int (length s) \<and> iss s w \<and> (\<forall>(s' :: int list). iss s' w \<longrightarrow> (1 :: int) \<le> int (length s') \<longrightarrow> s' ! (0 :: nat) < o1 + (1 :: int) \<longrightarrow> length s' \<le> length s) \<longrightarrow> len = int (length s) \<and> liss s w))) \<and> (o1 + (1 :: int) < (0 :: int) \<longrightarrow> (0 :: int) = int (length []) \<and> liss [] w)"
  sorry
end
